$\dbinom {n} {m} = \dbinom {n} {n-m}$

$\dbinom {n} {m} =\dbinom {n-1} {m-1} + \dbinom {n-1} m$

$(x+y)^n = \sum_{i=0}^n \dbinom {n} {i} x^i y^{n-i}$

$\sum_{i=0}^k \dbinom {n} {i} \dbinom {m} {k-i} = \dbinom {n+m} {k}$

$\dbinom {n} {m} \equiv \dbinom {n/p} {m/p} \times \dbinom {n \bmod p} {m \bmod p}\pmod p$

---

$\dbinom {n} {m} \times \dbinom {m} {k} = \dbinom {n} {k} \times \dbinom {n-k} {m-k}$

$\sum_{k=0}^m \dbinom {n+k} {k} = \dbinom {n+m+1} {m}$

$\dbinom {n} {m} \times m = \dbinom {n-1} {m-1} \times n$

$\dbinom {n} {k} \times (n-k) = \dbinom {n-1} {k} \times n$

$\dbinom {n} {m} = \dfrac {n \times (n-1) \times (n-2) \times  \dots (n-m+1)} {m!}  (a \in R)$

$\dbinom {n} {k} = (-1)^k \dbinom {k-n-1} {k}$

$\sum_{i=0}^k \dbinom {n} {i} (-1)^i = (-1)^k \dbinom {n-1} {k}$
